RHL_Typed.thy
@@ -226,6 +226,29 @@ unfolding rhoare_untyped
 apply (rule rtrans_rule[of _ P1 P2 Q1 Q2])
 using assms unfolding rhoare_untyped by auto
 
+
+
+lemma rtrans3_rule:
+  assumes p:"\<And>m1 m2. P m1 m2 \<Longrightarrow> \<exists>m m'. P1 m1 m \<and> P2 m m' \<and> P3 m' m2"
+      and q:"\<And>m1 m2 m m'. Q1 m1 m \<Longrightarrow> Q2 m m' \<Longrightarrow> Q3 m' m2 \<Longrightarrow> Q m1 m2"
+      and rhl1: "hoare {P1 &1 &2} \<guillemotleft>c1\<guillemotright> ~ \<guillemotleft>c2\<guillemotright> {Q1 &1 &2}"
+      and rhl2: "hoare {P2 &1 &2} \<guillemotleft>c2\<guillemotright> ~ \<guillemotleft>c3\<guillemotright> {Q2 &1 &2}"
+      and rhl3: "hoare {P3 &1 &2} \<guillemotleft>c3\<guillemotright> ~ \<guillemotleft>c4\<guillemotright> {Q3 &1 &2}"
+  shows "hoare {P &1 &2} \<guillemotleft>c1\<guillemotright> ~ \<guillemotleft>c4\<guillemotright> {Q &1 &2}"
+proof -
+  def Q12 == "\<lambda>m1 m'. \<exists>m. Q1 m1 m \<and> Q2 m m'"
+  def P12 == "\<lambda>m1 m'. \<exists>m. P1 m1 m \<and> P2 m m'"
+  have rhl12: "rhoare P12 c1 c3 Q12"
+    apply (rule rtrans_rule[OF _ _ rhl1 rhl2])
+    unfolding P12_def Q12_def by auto
+  show ?thesis
+    apply (rule rtrans_rule[OF _ _ rhl12 rhl3])
+    unfolding P12_def Q12_def
+     using p close metis
+    using q by metis
+qed
+
+
 lemma seq_assoc_left_rule: 
   assumes "hoare {P &1 &2} \<guillemotleft>a\<guillemotright>;\<guillemotleft>b\<guillemotright>;\<guillemotleft>c\<guillemotright> ~ \<guillemotleft>d\<guillemotright> {R &1 &2}"
   shows "hoare {P &1 &2} \<guillemotleft>a\<guillemotright>;{\<guillemotleft>b\<guillemotright>;\<guillemotleft>c\<guillemotright>} ~ \<guillemotleft>d\<guillemotright> {R &1 &2}"
@@ -508,6 +531,40 @@ lemma assertion_footprint_left_lookup: "mk_variable_untyped x \<in> X \<Longrigh
 lemma assertion_footprint_right_lookup: "mk_variable_untyped x \<in> X \<Longrightarrow> assertion_footprint_right X (\<lambda>m1 m2. memory_lookup m2 x)"
   unfolding assertion_footprint_right_def by auto
 
+
+lemma assertion_footprint_left_update:
+  assumes "Y \<subseteq> insert (mk_variable_untyped x) X"
+  assumes "assertion_footprint_left Y P"
+  shows "assertion_footprint_left X (\<lambda>m m'. P (memory_update m x v) m')"
+unfolding memory_update_def
+apply (rule assertion_footprint_left_update_untyped)
+using assms by auto
+
+lemma assertion_footprint_right_update:
+  assumes "Y \<subseteq> insert (mk_variable_untyped x) X"
+  assumes "assertion_footprint_right Y P"
+  shows "assertion_footprint_right X (\<lambda>m m'. P m (memory_update m' x v))"
+unfolding memory_update_def
+apply (rule assertion_footprint_right_update_untyped)
+using assms by auto
+
+
+lemma assertion_footprint_left_update_pattern:
+  assumes "Y \<subseteq> X \<union> set (p_vars pat)"
+  assumes "assertion_footprint_left Y P"
+  shows "assertion_footprint_left X (\<lambda>m m'. P (memory_update_pattern m pat x) m')"
+unfolding memory_update_pattern_def
+apply (rule assertion_footprint_left_update_pattern_untyped)
+using assms unfolding p_vars_def by auto
+
+lemma assertion_footprint_right_update_pattern:
+  assumes "Y \<subseteq> X \<union> set (p_vars pat)"
+  assumes "assertion_footprint_right Y P"
+  shows "assertion_footprint_right X (\<lambda>m m'. P m (memory_update_pattern m' pat x))"
+unfolding memory_update_pattern_def
+apply (rule assertion_footprint_right_update_pattern_untyped)
+using assms unfolding p_vars_def by auto
+
 lemma rskip_rule [simp]:
   assumes "\<forall>m m'. P m m' \<longrightarrow> Q m m'"
   shows "hoare {P &1 &2} skip ~ skip {Q &1 &2}"
@@ -702,5 +759,368 @@ lemma frame_rule:
 unfolding rhoare_untyped
 apply (rule frame_rule_untyped)
 using assms unfolding program_readonly_def program_untyped_readonly_def denotation_def rhoare_untyped by auto
+
+
+lemma callproc_equiv: 
+  assumes globals_V1: "set (vars_proc_global f) \<subseteq> V1"
+  assumes V2V1: "V2 \<subseteq> V1"
+  assumes x1V2: "set (p_vars x1) \<inter> V2 = {}"
+  assumes x2V2: "set (p_vars x2) \<inter> V2 = {}"
+  shows "rhoare (\<lambda>m1 m2. (\<forall>v\<in>V1. memory_lookup_untyped m1 v = memory_lookup_untyped m2 v)
+                      \<and> e_fun e1 m1 = e_fun e2 m2)
+                   (callproc x1 f e1) (callproc x2 f e2)
+                (\<lambda>m1 m2. (\<forall>v\<in>V2. memory_lookup_untyped m1 v = memory_lookup_untyped m2 v)
+                      \<and> memory_pattern_related x1 x2 m1 m2)"
+proof (rule rhoareI, goal_cases)
+case (1 m1 m2)  
+  hence eq_m1_m2: "memory_lookup_untyped m1 v = memory_lookup_untyped m2 v"
+        if "v\<in>V1" for v 
+    using that by auto
+  from 1 have e1e2: "e_fun e1 m1 = e_fun e2 m2" by simp
+  def argval == "e_fun e1 m1"
+  def m1a == "init_locals m1"
+  def m1b == "memory_update_pattern m1a (p_arg f) argval"
+  def m2a == "init_locals m2"
+  def m2b == "memory_update_pattern m2a (p_arg f) argval"
+
+  have eq_m12a: "memory_lookup_untyped m1a v = memory_lookup_untyped m2a v" if "v\<in>V1" for v 
+    using that eq_m1_m2 by (simp add: Rep_init_locals m1a_def m2a_def)
+  have eq_m12a_loc: "memory_lookup_untyped m1a v = memory_lookup_untyped m2a v" if "\<not> vu_global v" for v 
+    using that by (simp add: Rep_init_locals m1a_def m2a_def)
+  have eq_m12b_V1: "memory_lookup_untyped m1b v = memory_lookup_untyped m2b v" if "v\<in>V1" for v 
+    unfolding m1b_def m2b_def memory_update_pattern_def using that eq_m12a
+    by (metis lookup_memory_update_untyped_pattern_getter memory_lookup_update_pattern_notsame)
+  have eq_m12b_loc: "memory_lookup_untyped m1b v = memory_lookup_untyped m2b v" if "\<not> vu_global v" for v 
+    unfolding m1b_def m2b_def memory_update_pattern_def using eq_m12a_loc that
+    by (metis lookup_memory_update_untyped_pattern_getter memory_lookup_update_pattern_notsame)
+(*   have "memory_lookup_untyped m1b v = memory_lookup_untyped m2b v" if "v \<in> set(p_vars(p_arg f))" for v 
+    using that by auto *)
+
+  def V1loc == "V1 \<union> {x. \<not> vu_global x}"
+
+  have vars_V1loc: "set(vars(p_body f)) \<subseteq> V1loc"
+    using globals_V1 unfolding vars_proc_global_def V1loc_def by auto
+  with eq_m12b_V1 eq_m12b_loc
+  have eq_m12b: "memory_lookup_untyped m1b v = memory_lookup_untyped m2b v" if "v \<in> V1loc" for v
+    using that V1loc_def by auto
+
+  have "obs_eq V1loc V1loc (p_body f) (p_body f)"
+    unfolding obs_eq_obs_eq_untyped
+    apply (rule self_obseq_vars)
+    using vars_V1loc by (simp_all add: vars_def) 
+  
+  then obtain \<mu> where \<mu>fst: "apply_to_distr fst \<mu> = denotation (p_body f) m1b"
+                  and \<mu>snd: "apply_to_distr snd \<mu> = denotation (p_body f) m2b"
+                  and \<mu>post: "\<And>m1' m2' x. (m1',m2') \<in> support_distr \<mu> \<Longrightarrow> x\<in>V1loc \<Longrightarrow> 
+                                memory_lookup_untyped m1' x = memory_lookup_untyped m2' x"
+    unfolding obs_eq_def rhoare_def
+    using eq_m12b by blast 
+
+  def finalize == "\<lambda>m x. \<lambda>m'. let res = e_fun (p_return f) m'; m' = restore_locals m m' in memory_update_pattern m' x res"
+
+  def \<mu>' == "apply_to_distr (\<lambda>(m1',m2'). (finalize m1 x1 m1', finalize m2 x2 m2')) \<mu>"
+
+  have "apply_to_distr fst \<mu>' = apply_to_distr (\<lambda>m1'. finalize m1 x1 m1') (apply_to_distr fst \<mu>)"
+    unfolding \<mu>'_def by (simp add: split_def)
+  also have "\<dots> = apply_to_distr (\<lambda>m1'. finalize m1 x1 m1') (denotation (p_body f) m1b)"
+    using \<mu>fst by simp
+  also have "\<dots> = denotation (callproc x1 f e1) m1"
+    unfolding argval_def m1a_def m1b_def finalize_def
+    apply (subst denotation_callproc) by auto
+  finally have \<mu>'fst: "apply_to_distr fst \<mu>' = denotation (callproc x1 f e1) m1" by assumption
+
+  have "apply_to_distr snd \<mu>' = apply_to_distr (\<lambda>m2'. finalize m2 x2 m2') (apply_to_distr snd \<mu>)"
+    unfolding \<mu>'_def by (simp add: split_def)
+  also have "\<dots> = apply_to_distr (\<lambda>m2'. finalize m2 x2 m2') (denotation (p_body f) m2b)"
+    using \<mu>snd by simp
+  also have "\<dots> = denotation (callproc x2 f e2) m2"
+    unfolding argval_def m2a_def m2b_def finalize_def e1e2
+    apply (subst denotation_callproc) by auto
+  finally have \<mu>'snd: "apply_to_distr snd \<mu>' = denotation (callproc x2 f e2) m2"
+    by assumption
+
+  have \<mu>'post: "\<And>x. x\<in>V2 \<Longrightarrow> memory_lookup_untyped m1' x = memory_lookup_untyped m2' x"
+   and \<mu>'post2: "memory_pattern_related x1 x2 m1' m2'"
+               if supp: "(m1',m2') \<in> support_distr \<mu>'" 
+               for m1' m2'
+  proof -
+    from supp obtain m1'' m2'' where 
+        m1': "m1' = finalize m1 x1 m1''" and m2': "m2' = finalize m2 x2 m2''" and "(m1'',m2'') \<in> support_distr \<mu>"
+        unfolding \<mu>'_def by auto
+    hence eq_m12'': "\<And>x. x\<in>V1loc \<Longrightarrow> memory_lookup_untyped m1'' x = memory_lookup_untyped m2'' x"
+      using \<mu>post by simp
+
+    have ret_V1loc: "set (e_vars (p_return f)) \<subseteq> V1loc"
+      unfolding V1loc_def using globals_V1 unfolding vars_proc_global_def by auto
+    have ret12: "e_fun (p_return f) m1'' = e_fun (p_return f) m2''"
+      apply (rule e_fun_footprint)
+      apply (rule eq_m12'') 
+      using ret_V1loc by auto
+
+    show "memory_pattern_related x1 x2 m1' m2'"
+      apply (rule memory_pattern_relatedI)
+      unfolding m1' m2' finalize_def ret12 by auto
+
+    show "memory_lookup_untyped m1' x = memory_lookup_untyped m2' x" if "x\<in>V2" for x
+    proof -
+      def ret == "e_fun (p_return f) m1''"
+      def m1l == "restore_locals m1 m1''"
+      def m2l == "restore_locals m2 m2''"
+      have "m1' = memory_update_pattern m1l x1 ret"
+        unfolding ret_def m1' finalize_def m1l_def by auto
+      have "m2' = memory_update_pattern m2l x2 ret"
+        unfolding ret_def m2' finalize_def m2l_def ret12 by auto
+
+      have xx1: "x \<notin> set (p_vars x1)" and xx2: "x \<notin> set (p_vars x2)"
+        using x1V2 x2V2 that by auto
+
+      have "memory_lookup_untyped m1 x = memory_lookup_untyped m2 x"
+        using V2V1 eq_m1_m2 that by blast
+      moreover have "memory_lookup_untyped m1'' x = memory_lookup_untyped m2'' x"
+        using V1loc_def V2V1 eq_m12'' that by auto
+      ultimately have "memory_lookup_untyped (restore_locals m1 m1'') x = memory_lookup_untyped (restore_locals m2 m2'') x" 
+        unfolding Rep_restore_locals by simp
+
+      then have "memory_lookup_untyped (memory_update_pattern (restore_locals m1 m1'') x1 ret) x =
+                 memory_lookup_untyped (memory_update_pattern (restore_locals m2 m2'') x2 ret) x"
+        unfolding memory_update_pattern_def
+        apply (subst memory_lookup_update_pattern_notsame) close (metis p_vars_def xx1)
+        apply (subst memory_lookup_update_pattern_notsame) close (metis p_vars_def xx2)
+        by assumption
+      then show ?thesis
+        unfolding m1' m2' finalize_def ret_def[symmetric] ret12[symmetric] by simp
+    qed
+  qed
+
+  from \<mu>'fst \<mu>'snd \<mu>'post \<mu>'post2 show ?case
+    apply (rule_tac exI[of _ \<mu>']) by auto
+qed
+
+
+
+lemma call_rule:
+  fixes globals_f1 globals_f2 and x1::"'x1::prog_type pattern" and x2::"'x2::prog_type pattern" 
+    and y1::"'y1::prog_type expression" and y2::"'y2::prog_type expression" 
+    and res1::"'x1 variable" and res2::"'x2 variable" and A B P Q 
+  assumes globals_f1: "set(write_vars_proc_global f1) \<subseteq> set globals_f1"
+  assumes globals_f2: "set(write_vars_proc_global f2) \<subseteq> set globals_f2"
+  assumes args1_nin_f1: "mk_variable_untyped args1 \<notin> set (vars_proc_global f1)"
+  assumes args2_nin_f2: "mk_variable_untyped args2 \<notin> set (vars_proc_global f2)"
+  assumes footQ1: "assertion_footprint_left (-{mk_variable_untyped args1}) Q"
+  assumes footQ2: "assertion_footprint_right (-{mk_variable_untyped args2}) Q"
+  assumes f1f2: "rhoare P
+              (callproc (variable_pattern res1) f1 (var_expression args1))
+              (callproc (variable_pattern res2) f2 (var_expression args2))
+              Q"
+  defines "QB == (\<lambda>m1 m2. (\<forall>gL gR xL xR x'L x'R. 
+                     Q (memory_update (memory_update_untyped_pattern (memory_update_untyped_pattern m1 (list_pattern_untyped globals_f1) gL) (list_pattern_untyped (p_vars x1)) x'L) res1 xL)
+                       (memory_update (memory_update_untyped_pattern (memory_update_untyped_pattern m2 (list_pattern_untyped globals_f2) gR) (list_pattern_untyped (p_vars x2)) x'R) res2 xR)
+                \<longrightarrow> B (memory_update_pattern (memory_update_untyped_pattern m1 (list_pattern_untyped globals_f1) gL) x1 xL)
+                      (memory_update_pattern (memory_update_untyped_pattern m2 (list_pattern_untyped globals_f2) gR) x2 xR)))"
+  defines "C == (\<lambda>m1 m2. P (memory_update m1 args1 (e_fun y1 m1)) (memory_update m2 args2 (e_fun y2 m2)) \<and> QB m1 m2)"
+  assumes p1p2: "rhoare A p1 p2 C"
+  shows "rhoare A (seq p1 (callproc x1 f1 y1)) (seq p2 (callproc x2 f2 y2)) B"
+proof -
+
+(* Proof plan: 
+
+- Show:  rhoare    P{args/y}  (callproc x=f(y))  Q{x/res}    (substitution)   \<longrightarrow>  rhoareP'Q'
+- Show:  footprint QB   disjoint of   callproc x=f(y)
+- Show:  rhoare    C=P{args/y}\<and>QB     (callproc x=f(y))   Q{res/x}\<and>QB   (frame_rule) \<longrightarrow> rhoareQB
+- Show:  Q{res/x} \<and> QB \<Longrightarrow> B
+- Show:  rhoare    C     (callproc x=f(y))   B    (conseq)
+- Show:  rhoare    A     (p; callproc x=f(y))   B    (seq with assm)
+
+*)
+  def P' == "\<lambda>m1 m2. P (memory_update m1 args1 (e_fun y1 m1)) (memory_update m2 args2 (e_fun y2 m2))"
+  def x1l == "list_pattern_untyped (p_vars x1)"
+  def x2l == "list_pattern_untyped (p_vars x2)"
+  def Q' == "\<lambda>m1 m2. (\<exists>res1_val res2_val x1_val x2_val. 
+      memory_update_pattern m1 x1 res1_val = m1 \<and> memory_update_pattern m2 x2 res2_val = m2 \<and>
+      Q (memory_update (memory_update_untyped_pattern m1 x1l x1_val) res1 res1_val) (memory_update (memory_update_untyped_pattern m2 x2l x2_val) res2 res2_val))"
+
+  def VV1 == "- {mk_variable_untyped args1}"
+  def VV2 == "UNIV - {mk_variable_untyped args1, mk_variable_untyped res1} - set(p_vars x1)"
+  def VV1' == "- {mk_variable_untyped args2}"
+  def VV2' == "UNIV - {mk_variable_untyped args2, mk_variable_untyped res2} - set(p_vars x2)"
+
+  have y1_VV1: "mk_variable_untyped (args1::'y1 variable) \<notin> VV1" unfolding VV1_def by simp
+  have vv1_1: "set (vars_proc_global f1) \<subseteq> VV1" unfolding VV1_def using args1_nin_f1 by auto
+
+  have y2_VV1': "mk_variable_untyped (args2::'y2 variable) \<notin> VV1'" unfolding VV1'_def by simp
+  have x1: "set (vars_proc_global f2) \<subseteq> VV1'" unfolding VV1'_def using args2_nin_f2 by auto
+
+  have vv1_2: "VV2 \<subseteq> VV1" unfolding VV2_def VV1_def by auto
+  have x1_vv2: "set (p_vars x1) \<inter> VV2 = {}" unfolding VV2_def by auto
+  have res_vv2: "set (p_vars (variable_pattern res1 :: 'x1 pattern)) \<inter> VV2 = {}" unfolding VV2_def by auto
+
+  have x2: "VV2' \<subseteq> VV1'" unfolding VV2'_def VV1'_def by auto
+  have x3: "set (p_vars (variable_pattern res2 :: 'x2 pattern)) \<inter> VV2' = {}" unfolding VV2'_def by auto
+  have x4: "set (p_vars x2) \<inter> VV2' = {}" unfolding VV2'_def by auto
+
+  have foot_Q1: "assertion_footprint_left (insert (mk_variable_untyped (res1::'x1 variable)) VV2 \<union> set(p_vars x1)) Q" 
+    apply (rule assertion_footprint_left_mono[OF _ footQ1]) unfolding VV2_def by auto
+
+  have foot_Q2: "assertion_footprint_right (insert (mk_variable_untyped (res2::'x2 variable)) VV2' \<union> set(p_vars x2)) Q"
+    apply (rule assertion_footprint_right_mono[OF _ footQ2]) unfolding VV2'_def by auto
+
+  have x1_f1_res_f1: "hoare {\<lambda>m1 m2. (\<forall>v\<in>VV1. memory_lookup_untyped m1 v = memory_lookup_untyped m2 v) \<and> e_fun y1 m1 = e_fun (var_expression args1) m2}
+          \<guillemotleft>callproc x1 f1 y1\<guillemotright> ~ \<guillemotleft>callproc (variable_pattern res1) f1 (var_expression args1)\<guillemotright>
+        {\<lambda>m1 m2. (\<forall>v\<in>VV2. memory_lookup_untyped m1 v = memory_lookup_untyped m2 v) \<and> memory_pattern_related x1 (variable_pattern res1) m1 m2}"
+    apply (rule callproc_equiv)
+    using vv1_1 vv1_2 x1_vv2 res_vv2 by auto
+
+  have res_f2_x2_f2: "hoare {\<lambda>m1 m2. (\<forall>v\<in>VV1'. memory_lookup_untyped m1 v = memory_lookup_untyped m2 v) \<and> e_fun (var_expression args2) m1 = e_fun y2 m2}
+        \<guillemotleft>callproc (variable_pattern res2) f2 (var_expression args2)\<guillemotright> ~ \<guillemotleft>callproc x2 f2 y2\<guillemotright> 
+          {\<lambda>m1 m2. (\<forall>v\<in>VV2'. memory_lookup_untyped m1 v = memory_lookup_untyped m2 v) \<and> memory_pattern_related (variable_pattern res2) x2 m1 m2}"
+    apply (rule callproc_equiv)
+    using x1 x2 x3 x4 by auto
+
+  have t3: "\<exists>m m'. ((\<forall>v\<in>VV1. memory_lookup_untyped m1 v = memory_lookup_untyped m v) \<and>
+                     e_fun y1 m1 = e_fun (var_expression args1) m) \<and>
+                    P m m' \<and>
+                    (\<forall>v\<in>VV1'. memory_lookup_untyped m' v = memory_lookup_untyped m2 v) \<and> e_fun (var_expression args2) m' = e_fun y2 m2"
+                    if "P' m1 m2" for m1 m2
+    apply (rule exI[of _ "memory_update m1 args1 (e_fun y1 m1)"], rule exI[of _ "memory_update m2 args2 (e_fun y2 m2)"])
+    using y1_VV1 y2_VV1' that unfolding P'_def by simp
+
+  have t4: "Q' m1 m2"
+       if eq2: "\<forall>v\<in>VV2'. memory_lookup_untyped m' v = memory_lookup_untyped m2 v" 
+       and res_x2: "memory_pattern_related (variable_pattern res2) x2 m' m2" 
+       and eq1: "\<forall>v\<in>VV2. memory_lookup_untyped m1 v = memory_lookup_untyped m v" 
+       and x1_res: "memory_pattern_related x1 (variable_pattern res1) m1 m"
+       and "Q m m'" for m1 m2 m m'
+  proof -
+    def res1_val == "memory_lookup m res1 :: 'x1"
+    def res2_val == "memory_lookup m' res2 :: 'x2"
+    def x1_val == "eu_fun (list_expression_untyped (p_vars x1)) m"
+    def x2_val == "eu_fun (list_expression_untyped (p_vars x2)) m'"
+
+    from x1_res
+    obtain v where x1_v: "m1 = memory_update_pattern m1 x1 v" and res_v: "m = memory_update_pattern m (variable_pattern res1) v"
+      unfolding memory_pattern_related_def by auto
+    have "v = res1_val" unfolding res1_val_def apply (subst res_v) by simp
+    have x1_res1_val: "memory_update_pattern m1 x1 res1_val = m1" using x1_v `v=res1_val` by simp
+
+    from res_x2
+    obtain w where res_w: "m' = memory_update_pattern m' (variable_pattern res2) w" and x2_w: "m2 = memory_update_pattern m2 x2 w"
+      unfolding memory_pattern_related_def by auto
+    have "w = res2_val" unfolding res2_val_def apply (subst res_w) by simp
+    have x2_res2_val: "memory_update_pattern m2 x2 res2_val = m2" using x2_w `w=res2_val` by simp
+
+    have "Q (memory_update (memory_update_untyped_pattern m1 x1l x1_val) res1 res1_val) (memory_update (memory_update_untyped_pattern m2 x2l x2_val) res2 res2_val) = Q m (memory_update (memory_update_untyped_pattern m2 x2l x2_val) res2 res2_val)"
+      apply (rule assertion_footprint_leftE[OF foot_Q1])
+      using res1_val_def eq1 apply auto
+       close (metis list_pattern_untyped_list_expression_untyped lookup_memory_update_untyped_pattern_getter memory_lookup_update_pattern_notsame x1_val_def x1l_def)
+      by (metis list_pattern_untyped_list_expression_untyped lookup_memory_update_untyped_pattern_getter pu_vars_list_pattern_untyped x1_val_def x1l_def) 
+    also have "\<dots> = Q m m'"
+      apply (rule assertion_footprint_rightE[OF foot_Q2])
+      using res2_val_def eq2 apply auto
+       close (metis list_pattern_untyped_list_expression_untyped lookup_memory_update_untyped_pattern_getter memory_lookup_update_pattern_notsame x2_val_def x2l_def)
+      by (metis list_pattern_untyped_list_expression_untyped lookup_memory_update_untyped_pattern_getter pu_vars_list_pattern_untyped x2_val_def x2l_def) 
+  finally have Q': "Q (memory_update (memory_update_untyped_pattern m1 x1l x1_val) res1 res1_val)  
+                      (memory_update (memory_update_untyped_pattern m2 x2l x2_val) res2 res2_val)"
+    using that by simp                      
+
+    from Q' x1_res1_val x2_res2_val show ?thesis unfolding Q'_def by auto
+  qed
+
+  have rhoareP'Q': "rhoare P' (callproc x1 f1 y1) (callproc x2 f2 y2) Q'"
+    apply (rule rtrans3_rule[OF _ _ x1_f1_res_f1 f1f2 res_f2_x2_f2])
+     close (rule t3, simp)
+    by (rule t4, simp_all)
+
+  have foot_QB1: "assertion_footprint_left (UNIV - set globals_f1 - set (p_vars x1)) QB"
+    unfolding QB_def
+    apply (rule assertion_footprint_left_forall)+
+    apply (rule assertion_footprint_left_op2[where f="op\<longrightarrow>"])
+     apply (rule assertion_footprint_left_update_pattern_untyped[where Y="UNIV - set (p_vars x1)"])
+      close (simp, blast)
+     apply (rule assertion_footprint_left_update_pattern_untyped[where Y="UNIV"])
+      close simp
+     apply (rule assertion_footprint_left_update[where Y="UNIV"])
+      close
+     close (rule assertion_footprint_left_UNIV)
+    apply (rule assertion_footprint_left_update_pattern_untyped[where Y="UNIV - set (p_vars x1)"])
+     close (simp, blast)
+    apply (rule assertion_footprint_left_update_pattern[where Y="UNIV"])
+     close simp
+    by (rule assertion_footprint_left_UNIV)
+
+  have foot_QB2: "assertion_footprint_right (UNIV - set globals_f2 - set (p_vars x2)) QB"
+    unfolding QB_def
+    apply (rule assertion_footprint_right_forall)+
+    apply (rule assertion_footprint_right_op2[where f="op\<longrightarrow>"])
+     apply (rule assertion_footprint_right_update_pattern_untyped[where Y="UNIV - set (p_vars x2)"])
+      close (simp, blast)
+     apply (rule assertion_footprint_right_update_pattern_untyped[where Y="UNIV"])
+      close simp
+     apply (rule assertion_footprint_right_update[where Y="UNIV"])
+      close
+     close (rule assertion_footprint_right_UNIV)
+    apply (rule assertion_footprint_right_update_pattern_untyped[where Y="UNIV - set (p_vars x2)"])
+     close (simp, blast)
+    apply (rule assertion_footprint_right_update_pattern[where Y="UNIV"])
+     close simp
+    by (rule assertion_footprint_right_UNIV)
+    
+  have ro_f1: "program_readonly (UNIV - set globals_f1 - set (p_vars x1)) (callproc x1 f1 y1)"
+    apply (rule program_readonly_mono[rotated])
+     close (rule program_readonly_write_vars)
+    using globals_f1 by auto
+  have ro_f2: "program_readonly (UNIV - set globals_f2 - set (p_vars x2)) (callproc x2 f2 y2)"
+    apply (rule program_readonly_mono[rotated])
+     close (rule program_readonly_write_vars)
+    using globals_f2 by auto
+
+  have rhoareQB: "hoare {P' &1 &2 \<and> QB &1 &2} \<guillemotleft>callproc x1 f1 y1\<guillemotright> ~ \<guillemotleft>callproc x2 f2 y2\<guillemotright> {Q' &1 &2 \<and> QB &1 &2}"
+    apply (rule frame_rule)
+        close (fact foot_QB1)
+       close (fact foot_QB2)
+      close (fact ro_f1)
+     close (fact ro_f2)
+    by (fact rhoareP'Q')
+
+  have QB_Q: "B m1 m2" if Q'm1m2: "Q' m1 m2" and QBm1m2: "QB m1 m2" for m1 m2
+  proof -
+    from Q'm1m2 obtain res1_val res2_val x1_val x2_val
+      where ux1: "memory_update_pattern m1 x1 res1_val = m1"
+        and ux2: "memory_update_pattern m2 x2 res2_val = m2"
+        and Q: "Q (memory_update (memory_update_untyped_pattern m1 x1l x1_val) res1 res1_val) 
+                  (memory_update (memory_update_untyped_pattern m2 x2l x2_val) res2 res2_val)"
+      unfolding Q'_def by auto
+
+    def gL == "eu_fun (list_expression_untyped globals_f1) m1"
+    def gR == "eu_fun (list_expression_untyped globals_f2) m2"
+
+    have Q2: "Q (memory_update (memory_update_untyped_pattern (memory_update_untyped_pattern m1 (list_pattern_untyped globals_f1) gL) x1l x1_val) res1 res1_val)
+                (memory_update (memory_update_untyped_pattern (memory_update_untyped_pattern m2 (list_pattern_untyped globals_f2) gR) x2l x2_val) res2 res2_val)"
+      unfolding gL_def apply (subst list_pattern_untyped_list_expression_untyped)
+      unfolding gR_def apply (subst list_pattern_untyped_list_expression_untyped)
+      unfolding ux1 ux2 by (fact Q)
+
+    from QBm1m2[unfolded QB_def, folded x1l_def x2l_def, rule_format, of gL x1_val res1_val gR x2_val res2_val] 
+    have B2: "B (memory_update_pattern (memory_update_untyped_pattern m1 (list_pattern_untyped globals_f1) gL) x1 res1_val)
+                (memory_update_pattern (memory_update_untyped_pattern m2 (list_pattern_untyped globals_f2) gR) x2 res2_val)"
+    unfolding QB_def using that Q2 by simp
+
+    show "B m1 m2"
+      using B2
+      unfolding gL_def apply (subst (asm) list_pattern_untyped_list_expression_untyped)
+      unfolding gR_def apply (subst (asm) list_pattern_untyped_list_expression_untyped)
+      unfolding ux1 ux2 by simp
+  qed
+
+  have rhoareCQ: "hoare {C &1 &2} \<guillemotleft>callproc x1 f1 y1\<guillemotright> ~ \<guillemotleft>callproc x2 f2 y2\<guillemotright> {B &1 &2}"
+    apply (rule rconseq_rule[rotated -1])
+      close (fact rhoareQB)
+     unfolding C_def P'_def close
+    using QB_Q by auto
+
+  show ?thesis
+    apply (rule rseq_rule)
+     close (fact p1p2)
+    by (fact rhoareCQ)
+qed
 
 end
